through fixpoints

nominal_machine.lean
@@ -1,10 +1,19 @@
+import data.hash_map
+
 namespace nominal
 open list
 
 structure atom := (id : nat)
 namespace atom
 instance : decidable_eq atom := by tactic.mk_dec_eq_instance
+
 end atom
+
+def fresh_atom_core : list atom → ℕ → atom
+| [] next_id := ⟨next_id⟩
+| (atom::atoms) next_id := fresh_atom_core atoms (max atom^.id next_id)
+
+def fresh_atom (atoms : list atom) : atom := fresh_atom_core atoms 0
 
 inductive exp : Type
 | var : atom → exp
@@ -25,5 +34,59 @@ def swap (x y : atom) : exp → exp
 | (var z)     := var (swap_var x y z)
 | (abs z e)   := abs (swap_var x y z) (swap e)
 | (app e₁ e₂) := app (swap e₁) (swap e₂)
+
+def heap := hash_map atom (λ x, exp)
+structure frame := (val : exp)
+def stack := list frame
+
+structure config := (hp : heap) (t : exp) (stk : stack)
+
+inductive step (α : Type) : Type
+| error {} : step
+| done  {} : step
+| take     : α → step
+
+def machine_step (avoid : list atom) : config → step config
+| ⟨hp, abs x e, []⟩ := step.done
+
+| ⟨hp, abs x e, (⟨val⟩ :: stk)⟩ :=
+ if x ∈ hp^.keys ∪ avoid
+ then let y := fresh_atom (hp^.keys ∪ avoid) in step.take ⟨hp^.insert y val, swap x y e, stk⟩
+ else step.take ⟨hp^.insert x val, e, stk⟩
+
+| ⟨hp, var x, stk⟩ := match hp^.find x with
+                     | some e := step.take ⟨hp, e, stk⟩
+                     | none   := step.error
+                     end
+
+| ⟨hp, app f a, stk⟩ := step.take ⟨hp, f, ⟨a⟩ :: stk⟩
+
+def init_config (t : exp) : config := ⟨mk_hash_map (λ a : atom, a^.id), t, []⟩
+
+def is_val : exp → Prop
+| (abs _ _) := true
+| _         := false
+
+lemma values_are_done (avoid : list atom) : ∀ (t : exp), is_val t → machine_step avoid (init_config t) = step.done
+| (abs x e) _ := rfl
+| (var v) H_contra := false.rec _ H_contra
+| (app f a) H_contra := false.rec _ H_contra
+
+def size : exp → ℕ
+| (var x) := 1
+| (abs x e) := 1 + size e
+| (app f a) := 1 + size f + size a
+
+lemma swap_size_eq (x y : atom) : ∀ t, size (swap x y t) = size t :=
+begin
+intro t,
+induction t,
+reflexivity,
+all_goals { simp [swap, size], cc }
+end
+
+
+
+
 
 end nominal
