dce.lean
@@ -1,0 +1,210 @@
+import data.hash_map library_dev.data.list.set
+
+universe u
+
+namespace list
+
+def dnth {α : Type*} [decidable_eq α] [inhabited α] (xs : list α) (n : ℕ) : α :=
+match xs^.nth n with
+| (some x) := x
+| none     := default α
+end
+
+def at_nth {α : Type*} (xs : list α) (idx : ℕ) (x : α) : Prop := nth xs idx = some x
+
+def set_nth {α : Type*} : list α → ℕ → α → option (list α)
+| (x::xs) 0     a := some (a :: xs)
+| (x::xs) (i+1) a := do ys ← set_nth xs i a, return (x :: ys)
+| []      _     _ := none
+
+instance decidable_subset {α : Type*} [decidable_eq α] (xs ys : list α) : decidable (xs ⊆ ys) :=
+begin
+simp [has_subset.subset, list.subset],
+apply_instance
+end
+
+lemma at_nth_of_dnth_lt {α : Type*} [decidable_eq α] [inhabited α] {xs : list α} {idx : ℕ} :
+  idx < length xs → at_nth xs idx (dnth xs idx) := sorry
+
+lemma at_nth_of_len {α : Type*} {xs ys : list α} {x : α} {k : ℕ} : k = length xs → at_nth (xs ++ x :: ys) k x := sorry
+
+end list
+
+namespace hash_map
+
+def dfind {α : Type*} [decidable_eq α] {β : α → Type*} [∀ a, inhabited (β a)] (m : hash_map α β) (a : α) : β a :=
+match m^.find a with
+| (some b) := b
+| none     := default (β a)
+end
+
+end hash_map
+
+def hash_set (α : Type u) [decidable_eq α] : Type u :=
+hash_map α (λ x : α, unit)
+
+namespace hash_set
+
+variables {α : Type u} [decidable_eq α]
+
+def insert (s : hash_set α) (x : α) : hash_set α :=
+hash_map.insert s x ()
+
+def contains (s : hash_set α) (x : α) : bool :=
+(hash_map.find s x).is_some
+
+instance : has_mem α (hash_set α) := ⟨λa m, m.contains a⟩
+
+end hash_set
+
+section seq
+variables {α : Type*} (rel : α → α → Prop)
+
+inductive star : α → α → Prop
+| rfl    : ∀ (x : α), star x x
+| rtrans : ∀ (x y z : α), rel x y → star y z → star x y
+
+end seq
+
+namespace star
+variables {α : Type*} (rel : α → α → Prop)
+
+lemma trans (x y z : α) : star rel x y → star rel y z → star rel x z := sorry
+
+end star
+
+namespace compiler
+open tactic list
+
+structure var : Type := (id : ℕ)
+
+namespace var
+instance : decidable_eq var := by mk_dec_eq_instance
+end var
+
+@[reducible] def vstate : Type := hash_map var (λ v : var, ℕ)
+def empty_vstate : vstate := mk_hash_map (λ v : var, v^.id)
+
+inductive aexp : Type
+| aconst : ℕ → aexp
+| avar   : var → aexp
+| aadd   : aexp → aexp → aexp
+| asub   : aexp → aexp → aexp
+| amul   : aexp → aexp → aexp
+
+inductive bexp : Type
+| btrue  : bexp
+| bfalse : bexp
+| bnot   : bexp → bexp
+| band   : bexp → bexp → bexp
+| beq    : aexp → aexp → bexp
+| ble    : aexp → aexp → bexp
+
+def aeval (st : vstate) : aexp → ℕ
+| (aexp.aconst n) := n
+| (aexp.avar v) := st^.dfind v
+| (aexp.aadd e₁ e₂) := aeval e₁ + aeval e₂
+| (aexp.asub e₁ e₂) := aeval e₁ - aeval e₂
+| (aexp.amul e₁ e₂) := aeval e₁ * aeval e₂
+
+def beval (st : vstate) : bexp → bool
+| (bexp.btrue)      := tt
+| (bexp.bfalse)     := ff
+| (bexp.bnot b)     := bnot (beval b)
+| (bexp.band b₁ b₂) := beval b₁ && beval b₂
+| (bexp.beq e₁ e₂)  := aeval st e₁ = aeval st e₂
+| (bexp.ble e₁ e₂)  := aeval st e₁ ≤ aeval st e₂
+
+inductive com : Type
+| cskip  : com
+| cass   : var → aexp → com
+| cseq   : com → com → com
+| cif    : bexp → com → com → com
+| cwhile : bexp → com → com
+
+open com
+
+inductive ceval : com → vstate → vstate → Prop
+| eskip : ∀ st, ceval cskip st st
+| eass  : ∀ st a n x, aeval st a = n → ceval (cass x a) st (st^.insert x n)
+| eseq : ∀ c₁ c₂ st₁ st₂ st₃, ceval c₁ st₁ st₂ → ceval c₂ st₂ st₃ → ceval (cseq c₁ c₂) st₁ st₃
+| eift : ∀ st₁ st₂ b c₁ c₂, beval st₁ b = tt → ceval c₁ st₁ st₂ → ceval (cif b c₁ c₂) st₁ st₂
+| eiff : ∀ st₁ st₂ b c₁ c₂, beval st₁ b = ff → ceval c₂ st₁ st₂ → ceval (cif b c₁ c₂) st₁ st₂
+| ewhilet : ∀ st₁ st₂ st₃ b c, beval st₁ b = tt → ceval c st₁ st₂ → ceval (cwhile b c) st₂ st₃ → ceval (cwhile b c) st₁ st₃
+| ewhilef : ∀ st b c, beval st b = ff → ceval (cwhile b c) st st
+
+open ceval
+
+def fv_aexp : aexp → list var
+| (aexp.aconst n) := []
+| (aexp.avar v)   := [v]
+| (aexp.aadd e₁ e₂) := fv_aexp e₁ ∪ fv_aexp e₂
+| (aexp.asub e₁ e₂) := fv_aexp e₁ ∪ fv_aexp e₂
+| (aexp.amul e₁ e₂) := fv_aexp e₁ ∪ fv_aexp e₂
+
+def fv_bexp : bexp → list var
+| (bexp.btrue)      := []
+| (bexp.bfalse)     := []
+| (bexp.bnot b)     := fv_bexp b
+| (bexp.band b₁ b₂) := fv_bexp b₁ ∪ fv_bexp b₂
+| (bexp.beq e₁ e₂)  := fv_aexp e₁ ∪ fv_aexp e₂
+| (bexp.ble e₁ e₂)  := fv_aexp e₁ ∪ fv_aexp e₂
+
+def fv_com : com → list var
+| cskip         := []
+| (cass x e)    := fv_aexp e
+| (cseq c₁ c₂)  := fv_com c₁ ∪ fv_com c₂
+| (cif b c₁ c₂) := fv_bexp b ∪ fv_com c₁ ∪ fv_com c₂
+| (cwhile b c)  := fv_bexp b ∪ fv_com c
+
+section fixpoint
+
+parameter (F : list var → list var)
+parameter (dflt : list var)
+
+def iterate : ℕ → list var → list var
+| 0     _ := dflt
+| (n+1) x := let x' := F x in (if x' ⊆ x then x else iterate n x')
+
+lemma iterate_charact : ∀ (niter : ℕ) (start : list var), F (iterate niter start) ⊆ (iterate niter start) ∨ (iterate niter start) = dflt
+| 0           _     := or.inr rfl
+| (niter + 1) start :=
+begin
+simp only [iterate],
+have H_em : F start ⊆ start ∨ ¬ (F start ⊆ start) := decidable.em _,
+cases H_em with H_ss H_n_ss,
+{ simp only [H_ss, if_pos, if_simp_congr], left, triv },
+{ simp only [H_n_ss, if_neg, if_simp_congr, if_false], apply iterate_charact }
+end
+
+def fixpoint : list var := iterate 10 []
+
+lemma fixpoint_charact : (F fixpoint ⊆ fixpoint) ∨ (fixpoint = dflt) :=
+by apply iterate_charact
+
+variable (F_stable : ∀ x, x ⊆ dflt → F x ⊆ dflt)
+include F_stable
+
+lemma iterate_upper_bound : ∀ (niter : ℕ) (start : list var), start ⊆ dflt → iterate niter start ⊆ dflt
+| 0         start := by { simp [iterate] }
+| (niter+1) start :=
+begin
+simp [iterate],
+have H_em : F start ⊆ start ∨ ¬ (F start ⊆ start) := decidable.em _,
+cases H_em with H_ss H_n_ss,
+{ simp [H_ss], intro H, exact H },
+{ simp [H_n_ss], intro H, apply iterate_upper_bound, exact F_stable _ H }
+end
+
+lemma fixpoint_upper_bound : fixpoint ⊆ dflt :=
+begin
+apply iterate_upper_bound,
+exact F_stable,
+apply nil_subset
+end
+
+end fixpoint
+
+
+
+end compiler
